deps/poulet4/lib/CoqLib.v
@@ -1,0 +1,119 @@
+Require Import Coq.Arith.Arith.
+Require Import Coq.Strings.Ascii.
+Require Import Coq.Strings.String.
+Require Import Coq.Lists.List.
+Require Import Coq.micromega.Lia.
+
+Import ListNotations.
+
+Section mergeSort.
+
+  Variable A : Type.
+  Variable leb : A -> A -> bool.
+
+  Fixpoint insert (x : A) (ls : list A) : list A :=
+    match ls with
+    | nil => x :: nil
+    | h :: ls' => if leb x h then x :: ls else h :: insert x ls'
+    end.
+
+  Fixpoint merge (ls1 ls2 : list A) : list A :=
+    match ls1 with
+    | nil => ls2
+    | h :: ls' => insert h (merge ls' ls2)
+    end.
+
+  Fixpoint split (ls : list A) : list A * list A :=
+    match ls with
+    | nil => (nil, nil)
+    | h :: nil => (h :: nil, nil)
+    | h1 :: h2 :: ls' => let (ls1, ls2) := split ls' in (h1 :: ls1, h2 :: ls2)
+    end.
+
+  Definition lengthOrder (ls1 ls2 : list A) := length ls1 < length ls2.
+
+  Lemma lengthOrder_wf' : forall len, forall ls,
+        length ls <= len -> Acc lengthOrder ls.
+  Proof.
+    induction len; intros; constructor; intros; unfold lengthOrder in * |-.
+    - exfalso. destruct ls.
+      + simpl in H0. destruct y; simpl in H0; inversion H0.
+      + simpl in H; inversion H.
+    - apply IHlen. lia.
+  Defined.
+
+  Theorem lengthOrder_wf : well_founded lengthOrder.
+  Proof. red; intro; eapply lengthOrder_wf'; eauto. Defined.
+  
+  Lemma split_wf : forall len ls,
+      2 <= length ls <= len
+      -> let (ls1, ls2) := split ls in lengthOrder ls1 ls /\ lengthOrder ls2 ls.
+  Proof.
+    unfold lengthOrder. induction len; intros.
+    - destruct H. pose proof (Nat.le_trans _ _ _ H H0). inversion H1.
+    - destruct H. destruct ls; simpl in H. 1: inversion H. destruct ls.
+      1: simpl in H; inversion H; inversion H2. simpl in H.
+      destruct (le_lt_dec 2 (length ls)).
+      + simpl in H0. assert (2 <= length ls <= len) by lia.
+        specialize (IHlen _ H1). simpl. destruct (split ls). simpl. lia.
+      + destruct ls. 1: simpl; split; auto. simpl in l. destruct ls.
+        1: simpl; split; auto. simpl in l.
+        destruct ls; simpl in l; inversion l; inversion H2; inversion H4.
+  Qed.
+
+  Ltac split_wf := intros ls ?; intros; generalize (@split_wf (length ls) ls);
+                   destruct (split ls); destruct 1.
+
+  Lemma split_wf1 : forall ls, 2 <= length ls -> lengthOrder (fst (split ls)) ls.
+  Proof. split_wf. split; auto. auto. Qed.
+
+  Lemma split_wf2 : forall ls, 2 <= length ls -> lengthOrder (snd (split ls)) ls.
+  Proof. split_wf. split; auto. auto. Qed.
+
+  Hint Resolve split_wf1 split_wf2: merge_sort.
+
+  Definition mergeSort : list A -> list A.
+  Proof.
+    refine (Fix lengthOrder_wf (fun _ => list A)
+                (fun (ls : list A)
+                     (mergeSort : forall ls' : list A,
+                         lengthOrder ls' ls -> list A) =>
+                   if le_lt_dec 2 (length ls)
+                   then let lss := split ls in
+                        merge (mergeSort (fst lss) _) (mergeSort (snd lss) _)
+                   else ls)); subst lss; eauto with merge_sort.
+  Defined.
+
+  Theorem mergeSort_eq : forall ls,
+      mergeSort ls =
+      if le_lt_dec 2 (length ls)
+      then let lss := split ls in
+           merge (mergeSort (fst lss)) (mergeSort (snd lss))
+      else ls.
+  Proof.
+    intros; apply (Fix_eq lengthOrder_wf (fun _ => list A)). intros.
+    destruct (le_lt_dec 2 (length x)); simpl; f_equal; auto.
+  Qed.
+  
+End mergeSort.
+
+Arguments mergeSort {_} _ _.
+
+
+Definition ascii_leb (c1 c2: ascii) := BinNat.N.leb (N_of_ascii c1) (N_of_ascii c2).
+
+Fixpoint string_leb (s1 s2: string) :=
+  match s1, s2 with
+  | EmptyString, EmptyString => true
+  | String c1 s1, String c2 s2 =>
+    if (c1 =? c2)%char then string_leb s1 s2 else ascii_leb c1 c2
+  | EmptyString, String _ _ => true
+  | String _ _, EmptyString => false
+  end.
+
+Eval vm_compute in string_leb "abcd" "abcde".
+
+Local Open Scope string_scope.
+
+Eval vm_compute in
+    mergeSort string_leb ["Bob"; "Alice"; "Tom"; "Jinn"; "Jin"; "Carol"].
